src/Folds.v
@@ -35,3 +35,40 @@ Section fold_left3_opt.
       | _ , _ , _ => None
     end.
 End fold_left3_opt.
+
+Section All2.
+  Variable X Y : Type.
+  Variable F : X -> Y -> bool.
+
+  Fixpoint all2 (xs : list X) (ys : list Y) : bool :=
+    match xs , ys with
+      | nil , nil => true
+      | x :: xs, y :: ys => if F x y then all2 xs ys else false
+      | _ , _ => false
+    end.
+  
+  Variable P : X -> Y -> Prop.
+  Inductive Forall2 : list X -> list Y -> Prop :=
+  | Forall2_nil : Forall2 nil nil
+  | Forall2_cons : forall l ls r rs,
+    P l r ->
+    Forall2 ls rs -> Forall2 (l :: ls) (r :: rs).
+
+  Hypothesis F_P : forall x y, F x y = true -> P x y.
+  
+  Theorem all2_Forall2 : forall a b,
+    all2 a b = true -> Forall2 a b.
+  Proof.
+    induction a; destruct b; simpl; intros; try congruence; try solve [ econstructor ].
+      specialize (@F_P a y). destruct (F a y); eauto; try congruence; econstructor; eauto.
+  Qed.
+
+  Hypothesis P_F : forall x y, P x y -> F x y = true.
+  
+  Theorem Forall2_all2 : forall a b,
+    Forall2 a b -> all2 a b = true.
+  Proof.
+    induction 1; simpl; auto.
+    rewrite P_F; auto.
+  Qed.
+End All2.    
